module Small-Slice.Semi-Lattice where

open import Data.Unit
open import Data.Empty
open import Data.Sum renaming (map to mapâŠ)
open import Data.Nat hiding (_âŠ”_)
open import Data.Product renaming (map to mapÃ—)

open import Relation.Binary.PropositionalEquality hiding ([_])
 
open import Small-Slice.Univ
open import Small-Slice.ND-functions




ğ•ŒSL-âˆ¨ : {X : Set} â†’ ğ•ŒSL X â†’ ğ•ŒSL X â†’ ğ•ŒSL X
ğ•ŒSL-âˆ¨ (I , f) (J , g) = (ğ•ŒâŠ I J) , (Î» {(injâ‚ i) â†’ f i ; (injâ‚‚ j) â†’ g j})

ğ•ŒSL-â„• : {X : Set} â†’ (X â†’ ğ•ŒSL X) â†’ â„• â†’ X â†’ ğ•ŒSL X
ğ•ŒSL-â„• f zero x = ğ•ŒâŠ¤ , Î» i â†’ x
ğ•ŒSL-â„• f (suc n) x = (ğ•ŒÎ£ (projâ‚ (f x) , Î» i â†’ projâ‚ (ğ•ŒSL-â„• f n (projâ‚‚ (f x) i)))) ,
  Î» {(i , j) â†’ projâ‚‚ (ğ•ŒSL-â„• f n (projâ‚‚ (f x) i)) j}

ğ•ŒSL-Ï‰ : {X : Set} â†’ (X â†’ ğ•ŒSL X) â†’ (X â†’ ğ•ŒSL X)
ğ•ŒSL-Ï‰ f x = (ğ•ŒÎ£ (ğ•Œâ„• , (Î» n â†’ projâ‚ (ğ•ŒSL-â„• f n x)))) , Î» {(n , i) â†’ projâ‚‚ (ğ•ŒSL-â„• f n x) i}


-- Monoid
ğ•ŒSL-âˆ¨-âŠ‚ : {X : Set} â†’ {aâ‚€ aâ‚ bâ‚€ bâ‚ : ğ•ŒSL X} â†’ (ğ•ŒSLâ†’ X aâ‚€ aâ‚) â†’ (ğ•ŒSLâ†’ X bâ‚€ bâ‚)
  â†’ (ğ•ŒSLâ†’ X (ğ•ŒSL-âˆ¨ aâ‚€ bâ‚€) (ğ•ŒSL-âˆ¨ aâ‚ bâ‚))
ğ•ŒSL-âˆ¨-âŠ‚ aâŠ‚ bâŠ‚ (injâ‚ i) = (injâ‚ (projâ‚ (aâŠ‚ i))) , projâ‚‚ (aâŠ‚ i)
ğ•ŒSL-âˆ¨-âŠ‚ aâŠ‚ bâŠ‚ (injâ‚‚ j) = (injâ‚‚ (projâ‚ (bâŠ‚ j))) , projâ‚‚ (bâŠ‚ j)

ğ•ŒSL-âˆ¨-luni : {X : Set} â†’ (a : ğ•ŒSL X) â†’ ğ•ŒSLâ†’ X (ğ•ŒSL-âˆ¨ ğ•ŒSL-âŠ¥ a) a
ğ•ŒSL-âˆ¨-luni a (injâ‚‚ i) = i , refl

ğ•ŒSL-âˆ¨-runi : {X : Set} â†’ (a : ğ•ŒSL X) â†’ ğ•ŒSLâ†’ X (ğ•ŒSL-âˆ¨ a ğ•ŒSL-âŠ¥) a
ğ•ŒSL-âˆ¨-runi a (injâ‚ i) = i , refl

ğ•ŒSL-âˆ¨-left : {X : Set} â†’ (a b : ğ•ŒSL X) â†’ ğ•ŒSLâ†’ X a (ğ•ŒSL-âˆ¨ a b)
ğ•ŒSL-âˆ¨-left a b i = (injâ‚ i) , refl

ğ•ŒSL-âˆ¨-right : {X : Set} â†’ (a b : ğ•ŒSL X) â†’ ğ•ŒSLâ†’ X b (ğ•ŒSL-âˆ¨ a b)
ğ•ŒSL-âˆ¨-right a b i = (injâ‚‚ i) , refl

ğ•ŒSL-âˆ¨-idem : {X : Set} â†’ (a : ğ•ŒSL X) â†’ ğ•ŒSLâ†’ X (ğ•ŒSL-âˆ¨ a a) a
ğ•ŒSL-âˆ¨-idem a (injâ‚ i) = i , refl
ğ•ŒSL-âˆ¨-idem a (injâ‚‚ i) = i , refl

ğ•ŒSL-âˆ¨-comm : {X : Set} â†’ (a b : ğ•ŒSL X) â†’ ğ•ŒSLâ†’ X (ğ•ŒSL-âˆ¨ a b) (ğ•ŒSL-âˆ¨ b a)
ğ•ŒSL-âˆ¨-comm a b (injâ‚ i) = injâ‚‚ i , refl
ğ•ŒSL-âˆ¨-comm a b (injâ‚‚ j) = injâ‚ j , refl

ğ•ŒSL-âˆ¨-asso : {X : Set} â†’ (a b c : ğ•ŒSL X)
  â†’ ğ•ŒSLâ†’ X (ğ•ŒSL-âˆ¨ (ğ•ŒSL-âˆ¨ a b) c) (ğ•ŒSL-âˆ¨ a (ğ•ŒSL-âˆ¨ b c))
ğ•ŒSL-âˆ¨-asso a b c (injâ‚ (injâ‚ i)) = (injâ‚ i) , refl
ğ•ŒSL-âˆ¨-asso a b c (injâ‚ (injâ‚‚ j)) = injâ‚‚ (injâ‚ j) , refl
ğ•ŒSL-âˆ¨-asso a b c (injâ‚‚ k) = injâ‚‚ (injâ‚‚ k) , refl

ğ•ŒSL-âˆ¨-asso' : {X : Set} â†’ (a b c : ğ•ŒSL X)
  â†’ ğ•ŒSLâ†’ X (ğ•ŒSL-âˆ¨ a (ğ•ŒSL-âˆ¨ b c)) (ğ•ŒSL-âˆ¨ (ğ•ŒSL-âˆ¨ a b) c)
ğ•ŒSL-âˆ¨-asso' a b c (injâ‚ i) = (injâ‚ (injâ‚ i)) , refl
ğ•ŒSL-âˆ¨-asso' a b c (injâ‚‚ (injâ‚ j)) = (injâ‚ (injâ‚‚ j)), refl
ğ•ŒSL-âˆ¨-asso' a b c (injâ‚‚ (injâ‚‚ k)) = (injâ‚‚ k) , refl


ğ•ŒSL-âˆ¨-supremum : {X : Set} â†’ (a b c : ğ•ŒSL X)
  â†’ (ğ•ŒSLâ†’ X a c) â†’ (ğ•ŒSLâ†’ X b c) â†’ (ğ•ŒSLâ†’ X (ğ•ŒSL-âˆ¨ a b) c)
ğ•ŒSL-âˆ¨-supremum a b c aâŠ‚c bâŠ‚c (injâ‚ i) = aâŠ‚c i
ğ•ŒSL-âˆ¨-supremum a b c aâŠ‚c bâŠ‚c (injâ‚‚ j) = bâŠ‚c j


-- powertheory axioms
ğ•ŒSL-âˆ¨-idemâ‰¡ : {X : Set} â†’ (a : ğ•ŒSL X) â†’ ğ•ŒSLâ‰¡ (ğ•ŒSL-âˆ¨ a a) a
ğ•ŒSL-âˆ¨-idemâ‰¡ (I , a) =
  ğ•ŒSL-âˆ¨-idem (I , a) ,
  (Î» i â†’ (injâ‚ i) , refl)

ğ•ŒSL-âˆ¨-commâ‰¡ : {X : Set} â†’ (a b : ğ•ŒSL X) â†’ ğ•ŒSLâ‰¡ (ğ•ŒSL-âˆ¨ a b) (ğ•ŒSL-âˆ¨ b a)
ğ•ŒSL-âˆ¨-commâ‰¡ a b = ğ•ŒSL-âˆ¨-comm a b , ğ•ŒSL-âˆ¨-comm b a 

ğ•ŒSL-âˆ¨-assoâ‰¡ : {X : Set} â†’ (a b c : ğ•ŒSL X)
  â†’ ğ•ŒSLâ‰¡ (ğ•ŒSL-âˆ¨ (ğ•ŒSL-âˆ¨ a b) c) (ğ•ŒSL-âˆ¨ a (ğ•ŒSL-âˆ¨ b c))
ğ•ŒSL-âˆ¨-assoâ‰¡ a b c = ğ•ŒSL-âˆ¨-asso a b c , ğ•ŒSL-âˆ¨-asso' a b c

ğ•ŒSL-âˆ¨-lower : {X : Set} â†’ (a b : ğ•ŒSL X) â†’ ğ•ŒSLâ†’ _ a (ğ•ŒSL-âˆ¨ a b)
ğ•ŒSL-âˆ¨-lower a b = ğ•ŒSL-âˆ¨-left a b



-- Enriched by structure
ğ•ŒHom-âŠ¥ : {X Y : Set} â†’ ğ•ŒHom X Y
ğ•ŒHom-âŠ¥ x = ğ•ŒSL-âŠ¥

ğ•ŒHom-âˆ¨ : {X Y : Set} â†’ (f f' : ğ•ŒHom X Y) â†’ ğ•ŒHom X Y
ğ•ŒHom-âˆ¨ f f' x = ğ•ŒSL-âˆ¨ (f x) (f' x)


ğ•ŒHom-âˆ¨-left : {X Y : Set} â†’ (f f' : ğ•ŒHom X Y) â†’ ğ•ŒHom-âŠ‚ f (ğ•ŒHom-âˆ¨ f f')
ğ•ŒHom-âˆ¨-left f f' x = ğ•ŒSL-âˆ¨-left (f x) (f' x)

ğ•ŒHom-âˆ¨-right : {X Y : Set} â†’ (f f' : ğ•ŒHom X Y) â†’ ğ•ŒHom-âŠ‚ f' (ğ•ŒHom-âˆ¨ f f')
ğ•ŒHom-âˆ¨-right f f' x = ğ•ŒSL-âˆ¨-right (f x) (f' x)

ğ•ŒHom-âˆ¨-supremum : {X Y : Set} â†’ (f f' g : ğ•ŒHom X Y)
  â†’ (ğ•ŒHom-âŠ‚ f g) â†’ (ğ•ŒHom-âŠ‚ f' g) â†’ (ğ•ŒHom-âŠ‚ (ğ•ŒHom-âˆ¨ f f') g)
ğ•ŒHom-âˆ¨-supremum f f' g p q x = ğ•ŒSL-âˆ¨-supremum (f x) (f' x) (g x) (p x) (q x)


